coq/FUN.v
@@ -1,0 +1,372 @@
+Add LoadPath "/home/greg/Research/closedforms/coq".
+
+Require Import Coq.Bool.Bool.
+Require Import Coq.Arith.Arith.
+Require Import Coq.Arith.EqNat.
+Require Import Coq.omega.Omega.
+Require Import Coq.Lists.List.
+Require Import Coq.omega.Omega.
+
+Require Import NewImp.
+
+
+Module Translation.
+Import IMPEval.
+
+Inductive gxp : Type :=
+  | GNum : nat -> gxp
+  | GLoc: loc -> gxp
+  | GObj: (total_map nat (option gxp)) -> gxp
+  | GMap : (total_map loc (option gxp)) -> gxp
+  | GHasField: gxp -> gxp -> gxp
+  | GGet : gxp -> gxp -> gxp
+  | GPut : gxp -> gxp -> gxp -> gxp
+
+  | GPlus : gxp -> gxp -> gxp
+  | GMinus : gxp -> gxp -> gxp
+  | GMult : gxp -> gxp -> gxp
+
+  | GBool : bool -> gxp
+  | GEq : gxp -> gxp -> gxp
+  | GLt : gxp -> gxp -> gxp
+  | GNot : gxp -> gxp
+
+  | GIf : gxp -> gxp -> gxp -> gxp
+  | GFixIndex : nat -> id -> gxp -> gxp.
+
+Definition fvalid : gxp := GLoc (LId (Id 0)). (* "$valid" *)
+Definition fdata :  gxp := GLoc (LId (Id 1)). (* "$data"  *)
+Definition ftpe :   gxp := GNum 0. (* "$tpe"   *)
+Definition fval :   gxp := GNum 1. (* "$val"   *)
+
+Definition tnat :   gxp := GNum 0.
+Definition tbool :  gxp := GNum 1.
+Definition tloc :   gxp := GNum 2.
+
+Definition GEmpty : gxp := GMap (fun k =>
+                           match k with
+                           | LId x => Some (GObj (t_empty None))
+                           | LNew p => None
+                           end).
+
+Definition OEmpty : gxp := GObj(t_empty None).
+
+Definition GNone :  gxp := GPut GEmpty fvalid (GBool false).
+Definition GSome a : gxp := GPut (GPut GEmpty fvalid (GBool true)) fdata a.
+
+Definition GMatch (scrutinee: gxp) (none: gxp) (some: gxp -> gxp): gxp :=
+  GIf (GGet scrutinee fvalid) (some (GGet scrutinee fdata)) none.
+
+Definition GVSelect (addr: gxp) (field: gxp): gxp :=
+  GIf (GHasField addr field) (GSome (GGet addr field)) GNone.
+
+Definition GVNum (a: gxp): gxp :=
+  GPut (GPut OEmpty ftpe tnat) fval a.
+
+Definition GVBool (a: gxp): gxp :=
+  GPut (GPut OEmpty ftpe tbool) fval a.
+
+Definition GVLoc (a: gxp): gxp :=
+  GPut (GPut OEmpty ftpe tloc) fval a.
+
+Definition sym_store := total_map (option gxp).
+
+Definition toNatG (v:gxp): gxp :=
+  GIf (GEq (GGet v ftpe) tnat) (GSome (GGet v fval)) GNone.
+
+Definition toBoolG (v:gxp): gxp :=
+  GIf (GEq (GGet v ftpe) tbool) (GSome (GGet v fval)) GNone.
+
+Definition toLocG (v:gxp): gxp :=
+  GIf (GEq (GGet v ftpe) tloc) (GSome (GGet v fval)) GNone.
+
+Notation "'LETG' x <-- e1 'IN' e2"
+   := (GMatch e1 GNone (fun x => e2))
+   (right associativity, at level 60).
+(* Notation "'LETG' x <--- e1 'IN' e2"
+   := (match e1 with
+         | Some (Some x) => e2
+         | Some None => Some None
+         | None => None
+       end)
+   (right associativity, at level 60). *)
+
+Notation "e1 '>>g=' e2"
+   := (GMatch e1 GNone e2)
+   (right associativity, at level 80).
+
+(* ---------- translation (exp only for now) --------- *)
+Fixpoint trans_exp (e: exp) (sto: gxp): gxp :=
+  match e with
+  (* | AId x => GGet sto x (* fixme: check error *) *)
+  | ELoc id => GSome (GVLoc (GLoc (LId id)))
+  | ENum n => GSome (GVNum (GNum n))
+  | EPlus a b =>  LETG a <-- trans_exp a sto >>g= toNatG IN
+                  LETG b <-- trans_exp b sto >>g= toNatG IN
+                  GSome (GVNum (GPlus a b))
+  | EMinus a b => LETG a <-- trans_exp a sto >>g= toNatG IN
+                  LETG b <-- trans_exp b sto >>g= toNatG IN
+                  GSome (GVNum (GMinus a b))
+  | EMult a b =>  LETG a <-- trans_exp a sto >>g= toNatG IN
+                  LETG b <-- trans_exp b sto >>g= toNatG IN
+                  GSome (GVNum (GMult a b))
+  | EBool b =>      GSome (GVBool (GBool b))
+  | EEq a b =>    LETG a <-- trans_exp a sto >>g= toNatG IN
+                  LETG b <-- trans_exp b sto >>g= toNatG IN
+                  GSome (GVBool (GEq a b))
+  | ELt a b =>    LETG a <-- trans_exp a sto >>g= toNatG IN
+                  LETG b <-- trans_exp b sto >>g= toNatG IN
+                  GSome (GVBool (GLt a b))
+  | EAnd a b =>   LETG a <-- trans_exp a sto >>g= toBoolG IN
+                  LETG b <-- trans_exp b sto >>g= toBoolG IN
+                  GSome (GVBool (GIf a b (GBool false)))
+  | ENeg a =>     LETG a <-- trans_exp a sto >>g= toBoolG IN
+                  GSome (GVBool (GNot a))
+  | EFieldRead s n =>
+                  LETG s' <-- trans_exp s sto >>g= toLocG IN
+                  LETG n' <-- trans_exp n sto >>g= toNatG IN
+                  LETG o <-- GVSelect sto s' IN
+                  GVSelect o n'
+  end.
+
+
+Fixpoint trans_loop (e: exp) (s: stmt) (sto: gxp) (c: path) (n: nat) (* How to use GFixIndex? *)
+    (evstmt : gxp -> path -> gxp) : gxp:=
+  match n with
+  | O => GSome sto
+  | S n' =>
+    LETG b <-- trans_exp e sto >>g= toBoolG IN
+    LETG sto' <-- trans_loop e s sto c n' evstmt IN 
+    GIf b (evstmt sto' (PWhile c n')) GNone
+  end.
+
+Fixpoint trans_stmts (s: stmt) (sto: gxp) (c: path) { struct s }: gxp :=
+  match s with
+  | x ::= ALLOC =>
+    GPut (GPut sto (GLoc (LNew c)) OEmpty) (GLoc (LId x)) (GPut OEmpty (GLoc (LId (Id 0))) (GLoc (LNew c)))
+  | e1[[e2]] ::= e3 =>
+    LETG l <-- trans_exp e1 sto >>g= toLocG IN
+    LETG n <-- trans_exp e2 sto >>g= toNatG IN
+    LETG v <-- trans_exp e3 sto IN
+    LETG o <-- GVSelect sto l IN
+    GPut sto l (GPut o n v)
+  | IF e THEN s1 ELSE s2 FI =>
+    LETG b <-- trans_exp e sto >>g= toBoolG IN
+    GIf b (trans_stmts s1 sto (PThen c)) (trans_stmts s2 sto (PElse c))
+  | WHILE cnd DO s END =>
+      trans_loop cnd s sto c 3 (fun sto' c' => trans_stmts s sto' c')
+  | s1 ;; s2 =>
+      LETG sto' <-- trans_stmts s1 sto (PFst c) IN
+      trans_stmts s2 sto' (PSnd c)
+  | SKIP => GSome sto
+  | SAbort => GNone
+  end.
+
+(* ---------- small-step rules for FUN ---------- *)
+
+Inductive value : gxp -> Prop :=
+| v_num : forall n, value (GNum n)
+| v_loc : forall l, value (GLoc l)
+| v_bool : forall b, value (GBool b)
+| v_obj: forall m, (forall x y, m x = Some y -> value y) -> value (GObj m)
+| v_sto: forall m, (forall x y, m x = Some y -> value y) -> value (GMap m).
+
+Reserved Notation " t '==>' t' " (at level 40).
+
+Fixpoint subst (x : id) (s : gxp) (t : gxp) : gxp :=
+  match t with
+  | GNum n => GNum n
+  | GBool b => GBool b
+  | GLoc (LId i) => if beq_id i x then s else t
+  | GLoc l => GLoc l
+  | GObj m => GObj m
+  | GMap m => GMap m
+  
+  | GHasField m i => GHasField (subst x s m) (subst x s i)
+  | GGet m i => GGet (subst x s m) (subst x s i)
+  | GPut m i v => GPut (subst x s m) (subst x s i) (subst x s v)
+
+  | GPlus a b => GPlus (subst x s a) (subst x s b)
+  | GMinus a b => GMinus (subst x s a) (subst x s b)
+  | GMult a b => GMult (subst x s a) (subst x s b)
+
+  | GEq a b => GEq (subst x s a) (subst x s b)
+  | GLt a b => GLt (subst x s a) (subst x s b)
+  | GNot a => GNot (subst x s a)
+
+  | GIf c a b => GIf (subst x s c) (subst x s a) (subst x s b)
+  | GFixIndex i l b => if beq_id x l then t else GFixIndex i l (subst x s b)
+  end.
+
+Inductive step : gxp -> gxp -> Prop :=
+  (* GPlus *)
+  | ST_PlusConstConst : forall n1 n2,
+          GPlus (GNum n1) (GNum n2)
+      ==> GNum (n1 + n2)
+  | ST_Plus1 : forall t1 t1' t2,
+        t1 ==> t1' ->
+        GPlus t1 t2 ==> GPlus t1' t2
+  | ST_Plus2 : forall v1 t2 t2',
+        value v1 ->
+        t2 ==> t2' ->
+        GPlus v1 t2 ==> GPlus v1 t2'
+  (* GMinus *)
+  | ST_MinusConstConst : forall n1 n2,
+          GMinus (GNum n1) (GNum n2)
+      ==> GNum (n1 - n2)
+  | ST_Minus1 : forall t1 t1' t2,
+        t1 ==> t1' ->
+        GMinus t1 t2 ==> GMinus t1' t2
+  | ST_Minus2 : forall v1 t2 t2',
+        value v1 ->
+        t2 ==> t2' ->
+        GMinus v1 t2 ==> GMinus v1 t2'
+  (* GMult *)
+  | ST_MultConstConst : forall n1 n2,
+          GMult (GNum n1) (GNum n2)
+      ==> GNum (n1 * n2)
+  | ST_Mult1 : forall t1 t1' t2,
+        t1 ==> t1' ->
+        GMult t1 t2 ==> GMult t1' t2
+  | ST_Mult2 : forall v1 t2 t2',
+        value v1 -> 
+        t2 ==> t2' ->
+        GMult v1 t2 ==> GMult v1 t2'
+
+  (* GEq *)
+  | ST_EqNumConstConst : forall n1 n2,
+          GEq (GNum n1) (GNum n2)
+      ==> GBool (n1 =? n2)
+  | ST_EqLocConstConst : forall l1 l2,
+          GEq (GLoc l1) (GLoc l2)
+      ==> GBool (beq_loc l1 l2)
+  | ST_Eq1 : forall t1 t1' t2,
+        t1 ==> t1' ->
+        GEq t1 t2 ==> GEq t1' t2
+  | ST_Eq2 : forall v1 t2 t2',
+        value v1 ->
+        t2 ==> t2' ->
+        GEq v1 t2 ==> GEq v1 t2'
+
+  (* GLt *)
+  | ST_LtConstConst : forall n1 n2,
+          GLt (GNum n1) (GNum n2)
+      ==> GBool (n1 <? n2)
+  | ST_Lt1 : forall t1 t1' t2,
+        t1 ==> t1' ->
+        GLt t1 t2 ==> GLt t1' t2
+  | ST_Lt2 : forall v1 t2 t2',
+        value v1 ->
+        t2 ==> t2' ->
+        GLt v1 t2 ==> GLt v1 t2'
+  
+  (* GNot *)
+  | ST_NotConst : forall b1,
+          GNot (GBool b1)
+      ==> GBool (negb b1)
+  | ST_Not : forall t1 t1',
+        t1 ==> t1' ->
+        GNot t1 ==> GNot t1'
+
+  (* GIf *)
+  | ST_IfCond : forall t1 t1' t2 t3,
+       t1 ==> t1' ->
+       GIf t1 t2 t3 ==> GIf t1' t2 t3
+  | ST_IfTrue : forall t2 t3,
+       GIf (GBool true) t2 t3 ==> t2
+  | ST_IfFalse : forall t2 t3,
+       GIf (GBool false) t2 t3 ==> t3
+
+  (* GFixIndex*)
+  | ST_FixIndex : forall i l t,
+       GFixIndex (i + 1) l t ==> GIf (subst l (GNum i) t) (GNum i) (GFixIndex (i + 1) l t)
+
+  (* GHasField *)
+  | ST_ObjHasFieldTrue : forall n m,
+       m n <> None ->
+       GHasField (GObj m) (GNum n) ==> GBool true
+  | ST_ObjHasFieldFalse : forall n m,
+       m n = None ->
+       GHasField (GObj m)(GNum n)  ==> GBool false
+  | ST_StHasFieldTrue : forall l m,
+       m l <> None ->
+       GHasField (GMap m) (GLoc l) ==> GBool true
+  | ST_StoHasFieldFalse : forall l m,
+       m l = None ->
+       GHasField (GMap m) (GLoc l) ==> GBool false
+  | ST_HasFieldKey : forall t1 t2 t2',
+       t2 ==> t2' ->
+       GHasField t1 t2 ==> GHasField t1 t2'
+  | ST_HasFieldValue : forall t1 t1' v2,
+       value v2 ->
+       t1 ==> t1' ->
+       GHasField t1 v2 ==> GHasField t1' v2
+  (* GGet *)
+  | ST_ObjGet : forall n m v,
+       m n = Some v ->
+       GGet (GObj m) (GNum n) ==> v
+  | ST_StoreGet : forall l m v,
+       m l = Some v ->
+       GGet (GMap m) (GLoc l) ==> v
+  | ST_GetKey : forall t1 t2 t2',
+       t2 ==> t2' ->
+       GGet t1 t2 ==> GGet t1 t2'
+  | ST_GetValue : forall t1 t1' v2,
+       value v2 -> 
+       t1 ==> t1' ->
+       GGet t1 v2 ==> GGet t1' v2
+  (* GPut *)
+  | ST_ObjPut : forall n m t3,
+       GPut (GObj m) (GNum n) t3 ==> GObj (t_update beq_nat m n (Some t3))
+  | ST_StorePut : forall l m t3,
+       GPut (GMap m) (GLoc l) t3 ==> GMap (t_update beq_loc m l (Some t3))
+  | ST_PutKey : forall t1 t2 t2' t3,
+       t2 ==> t2' ->
+       GPut t1 t2 t3 ==> GPut t1 t2' t3
+  | ST_PutValue : forall t1 t1' v2 t3,
+       value v2 ->
+       t1 ==> t1' ->
+       GPut t1 v2 t3 ==> GPut t1' v2 t3
+  where " t '==>' t' " := (step t t').
+
+Definition relation (X: Type) := X->X->Prop.
+
+Inductive multi {X:Type} (R: relation X) : relation X :=
+  | multi_refl  : forall (x : X), multi R x x
+  | multi_step : forall (x y z : X),
+                    R x y ->
+                    multi R y z ->
+                    multi R x z.
+
+Notation " t '==>*' t' " := (multi step t t') (at level 40).
+
+(* ----- equivalence between IMP and FUN ----- *)
+
+Inductive veq : val -> gxp -> Prop :=
+| VEQ_Num : forall n r,
+    r ==>* (GVNum (GNum n)) ->
+    veq (VNum n) r
+| VEQ_Bool : forall n r,
+    r ==>* (GVBool (GBool n)) ->
+    veq (VBool n) r
+| VEQ_Loc : forall l r,
+    r ==>* (GVLoc (GLoc l)) ->
+    veq (VLoc l) r.
+
+Inductive oeq {X:Type} (peq: X -> gxp -> Prop): option X -> gxp -> Prop :=
+| REQ_Some : forall v g r,
+    peq v g ->
+    r ==>* (GSome g) ->
+    oeq peq (Some v) r
+| REQ_None : forall r,
+    r ==>* GNone ->
+    oeq peq None r.
+
+Definition req := oeq veq.
+
+(* small-step: not currently used *)
+Theorem soundness1: forall e,
+    exists g, (trans_exp e (GEmpty)) ==> g \/ (value g /\ req (evalExp e (σ0)) g).
+Proof.
+
+End Translation.
